feat: hole defs are satisfied

Lean/Geo/WBPoints.lean
@@ -12,15 +12,15 @@ theorem nodup_of_gp (l : List Point) :
     3 < l.length → PointListInGeneralPosition l → l.Nodup :=
   sorry
 
-/-- A well-behaved list of points: in general position, sorted by `x`. -/
+/-- A well-behaved list of points: in general position, sorted by `x`,
+and containing at least one point `leftmost`
+such that all signotopes `σ leftmost a b` are `CCW`. -/
 structure WBPoints where
   leftmost : Point
   rest : List Point
-  sorted : PointListSorted (leftmost :: rest)
-  gp : PointListInGeneralPosition (leftmost :: rest)
+  sorted' : PointListSorted (leftmost :: rest)
+  gp' : PointListInGeneralPosition (leftmost :: rest)
   oriented : rest.Pairwise (σ leftmost · · = .CCW)
-
-def WBPoints.points (w : WBPoints) := w.leftmost :: w.rest
 
 def finset_sort (S : Finset Point) : List Point :=
   S.toList.insertionSort (·.x <= ·.x)
@@ -32,7 +32,15 @@ namespace WBPoints
 open List Finset Classical
 open LeanSAT Model PropFun
 
+def points (w : WBPoints) := w.leftmost :: w.rest
+
 def toFinset (w : WBPoints) : Finset Point := w.points.toFinset
+
+theorem sorted (w : WBPoints) : PointListSorted w.points :=
+  w.sorted'
+
+theorem gp (w : WBPoints) : PointListInGeneralPosition w.points :=
+  w.gp'
 
 theorem nodupX (w : WBPoints) : w.points.Pairwise (·.x ≠ ·.x) :=
   Pairwise.imp ne_of_lt w.sorted
@@ -45,9 +53,33 @@ abbrev length (w : WBPoints) : Nat := w.points.length
 instance : GetElem WBPoints Nat Point (fun w i => i < w.length) where
   getElem w i h := w.points[i]'h
 
+theorem sorted_get (w : WBPoints) {i j : Fin w.length} :
+    i < j → w[i].x < w[j].x := by
+  intro ij
+  apply List.pairwise_iff_get.mp w.sorted _ _ ij
+
+theorem of_sorted_get (w : WBPoints) {i j : Fin w.length} :
+    w[i].x < w[j].x → i < j := by
+  intro wiwj
+  by_contra h
+  rcases lt_or_eq_of_le (not_lt.mp h) with h | h
+  . have := w.sorted_get h
+    linarith
+  . rw [h] at wiwj
+    linarith
+
+theorem of_eqx (w : WBPoints) {i j : Fin w.length} :
+    w[i].x = w[j].x → i = j := by
+  intro h
+  by_contra h
+  rcases Ne.lt_or_lt h with h | h <;> {
+    have := w.sorted_get h
+    linarith
+  }
+
 -- TODO: use a definition from an earlier module
 def σIsEmptyTriangleFor (a b c : Point) (S : Finset Point) : Prop :=
-  ∀ s ∈ S \ {a,b,c}, ¬σPtInTriangle s a b c
+  ∀ s ∈ S, ¬σPtInTriangle s a b c
 
 def toPropAssn (w : WBPoints) : PropAssignment (Var w.length)
   | .sigma a b c ..    => σ w[a] w[b] w[c] = .CCW
@@ -136,8 +168,87 @@ theorem satisfies_insideDefs (w : WBPoints) : w.toPropAssn ⊨ insideDefs w.leng
       simp [abc.left, abc.left.trans bxc.left, abc.left.trans abc.right, bxc.left, abc.right, bxc.right]
     simp [-getElem_fin, insideDefs_aux₂ (w.sorted.to₄ this) (PointListInGeneralPosition.to₄ w.gp this)]
 
+lemma xBounded_of_PtInTriangle {x a b c : Point} :
+    Sorted₃ a b c → PtInTriangle x a b c → a.x ≤ x.x ∧ x.x ≤ c.x := by
+  unfold PtInTriangle
+  intro sorted tri
+  let S := { p : Point | a.x ≤ p.x } ∩ { p : Point | p.x ≤ c.x }
+  have cvxS : Convex ℝ S :=
+    Convex.inter
+      (convex_halfspace_ge ⟨fun _ _ => rfl, fun _ _ => rfl⟩ a.x)
+      (convex_halfspace_le ⟨fun _ _ => rfl, fun _ _ => rfl⟩ c.x)
+  have abcS : {a, b, c} ⊆ S := by
+    intro x hx
+    simp only [Set.mem_insert_iff, Set.mem_singleton_iff] at hx
+    simp only [Set.mem_inter_iff, Set.mem_setOf_eq]
+    rcases hx with rfl | rfl | rfl
+    . exact ⟨le_rfl, le_of_lt <| sorted.h₁.trans sorted.h₂⟩
+    . exact ⟨le_of_lt sorted.h₁, le_of_lt sorted.h₂⟩
+    . exact ⟨le_of_lt <| sorted.h₁.trans sorted.h₂, le_rfl⟩
+  have : x ∈ S := convexHull_min abcS cvxS tri
+  simpa only [Set.mem_inter_iff, Set.mem_setOf_eq] using this
+
+-- TODO: Use the real actual proof
+lemma σiff {x a b c : Point} : σPtInTriangle x a b c ↔ PtInTriangle x a b c := sorry
+
 theorem satisfies_holeDefs (w : WBPoints) : w.toPropAssn ⊨ holeDefs w.length := by
-  sorry -- TODO: we should agree on a defn of σIsEmptyTriangleFor globally first
+  unfold holeDefs notHoleOfPointInside hasPointInside
+  simp only [satisfies_all, Multiset.mem_map, forall_exists_index, forall_apply_eq_imp_iff, mem_val, mem_univ, true_and]
+  intro a b c
+  split_ifs <;> try exact satisfies_tr
+  simp only [ne_eq, satisfies_conj, satisfies_all, Multiset.mem_map, mem_val, mem_univ, true_and,
+    forall_exists_index, forall_apply_eq_imp_iff, satisfies_impl, satisfies_neg, satisfies_var,
+    Bool.not_eq_true, satisfies_any, exists_exists_eq_and]
+  constructor
+  . intro x
+    split_ifs <;> try exact satisfies_tr
+    simp only [satisfies_impl, satisfies_var, toPropAssn, decide_eq_true_eq, satisfies_neg,
+      σIsEmptyTriangleFor, not_forall, not_not, exists_prop, toFinset, List.mem_toFinset]
+    intro h
+    exact ⟨w[x], List.get_mem _ x _, h⟩
+  . intro h
+    simp only [toPropAssn, σIsEmptyTriangleFor, decide_eq_false_iff_not, not_forall,
+      not_not, exists_prop] at h
+    have ⟨x, hx, tri⟩ := h
+    rcases List.get_of_mem <| List.mem_toFinset.mp hx with ⟨i, rfl⟩
+    have : List.get w.points i = w[i] := rfl
+    rw [this] at tri hx
+    clear this
+    use i
+    split_ifs
+    . simp only [toPropAssn, satisfies_var, decide_eq_true_eq, tri]
+    next h =>
+      exfalso
+      simp only [not_and, not_not] at h
+      have sub : [w[a],w[b],w[c]] <+ w.points := by
+        have : [w[a],w[b],w[c]] = [a,b,c].map w.points.get := by
+          simp [GetElem.getElem, List.getElem_eq_get]
+        rw [this]
+        apply map_get_sublist
+        aesop (add unsafe lt_trans)
+      have ⟨wawi, wiwc⟩ := xBounded_of_PtInTriangle (w.sorted.to₃ sub) (σiff.mp tri)
+      have : i ≠ a := fun h => by
+        rw [h] at tri
+        have := not_mem_σPtInTriangle (w.gp sub).perm₁
+        have := tri.perm₁
+        contradiction
+      have : w[a].x < w[i].x := by
+        apply lt_of_le_of_ne wawi
+        intro h
+        exact this <| w.of_eqx h.symm
+      have ai : a < i := w.of_sorted_get this
+      have : i ≠ c := fun h => by
+        rw [h] at tri
+        have := not_mem_σPtInTriangle (w.gp sub).perm₂
+        have := tri.perm₂
+        contradiction
+      have : w[i].x < w[c].x := by
+        apply lt_of_le_of_ne wiwc
+        intro h
+        exact this <| w.of_eqx h
+      have ic : i < c := w.of_sorted_get this
+      rw [h ai ic] at tri
+      apply not_mem_σPtInTriangle (w.gp sub) tri
 
 theorem satisfies_leftmostCCWDefs (w : WBPoints) : w.toPropAssn ⊨ pointsCCW w.length := by
   sorry
